working var case completeness

src/Completeness.v
@@ -29,6 +29,44 @@ Ltac destructMatch :=
     | [ |- context[match ?a with  | _ => _ end] ] => destruct a
   end.
 
+Lemma assoc_subst_exists : forall (G : ctx) (i : id) (s : substitution) (sigma : schm),
+    in_ctx i (apply_subst_ctx s G) = Some sigma ->
+    {sigma' : schm | in_ctx i G = Some sigma' /\ sigma = apply_subst_schm s sigma'}.
+Proof.
+Admitted.
+
+Lemma in_ctx_look_def : forall i G sigma (ev : in_ctx i G = Some sigma),
+    look_dep i G = ret (exist _ sigma ev).
+Proof.
+  Admitted.
+
+Lemma list_ty_and_id_inv : forall lt_st : list ty * id,
+    {lt_st1 : list ty * id | lt_st1 = lt_st}.
+Proof.
+intros lt_st; exists lt_st; auto.
+Qed.
+
+Fixpoint compute_gen_subst (i : id) (n : nat) : (list ty) * id :=
+  match n with
+  | O => (nil, i)
+  | S p => match compute_gen_subst (S i) p with
+      | (l, i') => (var i :: l, i')
+      end
+  end.
+
+Fixpoint max_gen_vars (sigma : schm) : nat :=
+  match sigma with
+  | sc_con _ => 0
+  | sc_var _ => 0
+  | sc_gen i => S i
+  | sc_arrow s1 s2 => max (max_gen_vars s1) (max_gen_vars s2)
+  end.
+
+Lemma apply_compute_gen_subst : forall (i : id) (sigma : schm) (p : nat),
+    max_gen_vars sigma <= p ->
+    {tau : ty | apply_inst_subst (fst (compute_gen_subst i p)) sigma = Some_schm tau}.
+Admitted.
+
 Lemma completeness : forall (e : term) (G : ctx) (tau' : ty) (phi : substitution) (i : id),
     has_type (apply_subst_ctx phi G) e tau' -> new_tv_ctx G i ->
     exists s tau i' s', getResult (runInfer_id e G i) = Some (i', tau, s) /\
@@ -37,40 +75,33 @@ Lemma completeness : forall (e : term) (G : ctx) (tau' : ty) (phi : substitution
 Proof.
   intros.
   induction e.
-  admit.
-  admit.
-  admit.
-  admit.
   - unfold runInfer_id, getResult.
     inversion H.
     subst.
-    eapply has_type_is_stable_under_substitution_inversion_con in H.
-    induction G.
-    admit.
-    simpl in *.
-    destructMatch.
-    destructMatch.
-    destructMatch.
+    destruct (assoc_subst_exists G i0 phi H2).
+    destructs a.
+    pose proof in_ctx_look_def i0 G H1 as IN1. 
+    simpl.
+    destruct (list_ty_and_id_inv (compute_gen_subst i (max_gen_vars x))).
+    assert ((max_gen_vars x) <= i). admit.
+    destruct (apply_compute_gen_subst i x H5).
+
     destruct s.
     destruct s.
-    destruct a.
     inversion h.
-    inversion H.
     subst.
-    exists x0 (con i1) next_tvar (nil : substitution).
+    destruct (assoc_subst_exists G i0 x1 H6).
+    destructs a.
+    pose proof in_ctx_look_def i0 G H3 as IN2. 
+    exists x1 x0 next_tvar x1.
     splits.
     reflexivity.
-    simpl.
-    reflexivity.
 
+    simpl.
+    destruct sigma_dep.
     
-    destruct (look_const_dep i0 G).
-    admit.
-    auto.
-    simpl.
-    mysimp.
-    destruct const_dep.
-
-    split; try reflexivity.
-
-Admitted.
+  admit.
+  admit.
+  admit.
+  admit.
+  - admit.
